stdlib/ptr/output/ptr/proofs/proof_const_ptr_sub.v
@@ -1,0 +1,66 @@
+From caesium Require Import lang notation.
+From refinedrust Require Import typing shims.
+From stdlib.ptr.ptr.generated Require Import generated_code_ptr generated_specs_ptr generated_template_const_ptr_sub.
+
+Set Default Proof Using "Type".
+
+Section proof.
+Context `{RRGS : !refinedrustGS Σ}.
+
+Lemma const_ptr_sub_proof (π : thread_id) :
+  const_ptr_sub_lemma π.
+Proof.
+  const_ptr_sub_prelude.
+
+  repeat liRStep; liShow.
+  liFromSyntax.
+  iRename select (loc_in_bounds l _ _) into "Hbounds".
+  iDestruct "Hbounds" as "#Hbounds".
+  repeat liRStep; liShow.
+  rewrite /typed_bin_op/typed_val_expr.
+  iIntros "Hv1 Hv2" (Φ) "#CTX #HE HL Hcont".
+  rewrite {1}/ty_own_val /=. iDestruct "Hv1" as %[Hv1 Hsz1].
+  rewrite {1}/ty_own_val /=. iDestruct "Hv2" as "->".
+  iDestruct (loc_in_bounds_ptr_in_range with "Hbounds") as %[Hran1 Hran2].
+  rewrite /size_of_st. simplify_layout_goal.
+  iRename select (credit_store _ _) into "Hstore".
+  iPoseProof (credit_store_borrow_receipt with "Hstore") as "(Hat & Hatcl)".
+  iDestruct "CTX" as "(LFT & TIME & LLCTX)".
+  iMod (persistent_time_receipt_0) as "Hp".
+  iApply (wp_ptr_neg_offset_credits with "TIME Hat Hp").
+  { done. }
+  { apply val_to_of_loc. }
+  { done. }
+  { (* count is positive, so this should work *)
+    revert H30 H31.
+    split; rewrite -?MinInt_eq -?MaxInt_eq. 
+    { move: H31. unsafe_unfold_common_caesium_defs; simpl. lia. }
+    { lia. }
+  }
+  { rewrite /offset_loc.
+    iApply (loc_in_bounds_offset with "Hbounds").
+    { done. }
+    { destruct l; simpl. clear Hran2. lia. }
+    { destruct l; simpl. clear Hran1. lia. }
+  }
+  { iApply (loc_in_bounds_offset with "Hbounds"); [ done | | ].
+    { clear Hran2. lia. }
+    { clear Hran1. lia. }
+  }
+  iNext. simpl. iEval (rewrite additive_time_receipt_succ). iIntros "Hcred [Hat Hat']".
+  iPoseProof ("Hatcl" with "Hat'") as "Hstore".
+  iPoseProof (credit_store_donate with "Hstore Hcred") as "Hstore".
+  iPoseProof (credit_store_donate_atime with "Hstore Hat") as "Hstore".
+  iApply ("Hcont" $! _ π _ _ (alias_ptr_t) with "HL").
+  { rewrite /ty_own_val /=. done. }
+  iAssert ((l offset{use_layout_alg' (ty_syn_type T_ty)}ₗ count) ◁ᵥ{ π} l offset{use_layout_alg' (ty_syn_type T_ty)}ₗ count @ alias_ptr_t)%I as "?".
+  { rewrite /ty_own_val /= //. }
+
+  repeat liRStep; liShow.
+
+  all: print_remaining_goal.
+  Unshelve. all: sidecond_solver.
+  Unshelve. all: sidecond_hammer.
+  Unshelve. all: print_remaining_sidecond.
+Qed.
+End proof.
